\documentclass[unknownkeysallowed]{beamer}
\usepackage[french,english]{babel}
\usepackage{./sty/beamer_js}
\usepackage{./sty/shortcuts_js}
\usepackage{csquotes}


\addbibresource{Bibliographie.bib}
\usepackage{enumerate}

\begin{document}


%%%%%%%%%%%%%%%%%%%%%%%%%%%%%%%%%%%%%%%%%%%%%%%%%%%%%%%%%%%%%%%%%%%%%%%%%%%%%%%
%%%%%%%%%%%%%%%%%%%%%%             Headers               %%%%%%%%%%%%%%%%%%%%%%
%%%%%%%%%%%%%%%%%%%%%%%%%%%%%%%%%%%%%%%%%%%%%%%%%%%%%%%%%%%%%%%%%%%%%%%%%%%%%%%



%%%%%%%%%%%%%%%%%%%%%%%%%%%%%%%%%%%%%%%%%%%%%%%%%%%%%%%%%%%%%%%%%%%%%%%%%%%%%%%
\begin{frame}[noframenumbering]
\thispagestyle{empty}
\bigskip
\bigskip
\begin{center}{
\LARGE\color{marron}
\textbf{HMMA 307 : Advanced Linear Modeling}
\textbf{ }\\
\vspace{0.5cm}
}

\color{marron}
\textbf{Chapter 3 : ANOVA}
\end{center}

\vspace{0.5cm}

\begin{center}
\textbf{COIFFIER OPHELIE \ GAIZI IBRAHIM \ LEFORT TANGUY } \\
\vspace{0.1cm}
\url{https://github.com/opheliecoiffier/CM_Anova}\\
\vspace{0.5cm}
Université de Montpellier \\
\end{center}

\centering
\includegraphics[width=0.13\textwidth]{logo.png}
\end{frame}


%%%%%%%%%%%%%%%%%%%%%%%%%%%%%%%%%%%%%%%%%%%%%%%%%%%%%%%%%%%%%%%%%%%%%%%%%%%%%%%
%%%%%%%%%%%%%%%%%%%%%%%%%   table of contents     %%%%%%%%%%%%%%%%%%%%%%%%%%%%%
%%%%%%%%%%%%%%%%%%%%%%%%%%%%%%%%%%%%%%%%%%%%%%%%%%%%%%%%%%%%%%%%%%%%%%%%%%%%%%%

\begin{frame}[noframenumbering]
\thispagestyle{empty}
\tableofcontents
\end{frame}




\section{Statistical model for the ANOVA}

%%%%%%%%%%%%%%%%%%%%%%%%%%%%%%%%%%%%%%%%%%%%%%%%%%%%%%%%%%%%%%%%%%%%%%%%%%%%%%%
%%%%%%%%%%%%%%%%%%%%%%          ANOVA Model              %%%%%%%%%%%%%%%%%%%%%%
%%%%%%%%%%%%%%%%%%%%%%%%%%%%%%%%%%%%%%%%%%%%%%%%%%%%%%%%%%%%%%%%%%%%%%%%%%%%%%%

\begin{frame}{Statistical model}
\begin{alertblock}{Model equation}
\[y_{ij}=\mu_i^*+\varepsilon_{ij}\]
\end{alertblock}

\medskip

 \begin{itemize}
        \item $\varepsilon_{ij} \overset{\iid}{\sim} \mathcal{N}(0,\sigma^2) $ is the noise
and $\cov(\epsilon_{ij},\varepsilon_{i'j'})=\sigma^2 \delta_{ii'} \delta_{jj'} $
        \item $y_{ij}$ is the $j^{th}$ measure for the modality
        \item $\bar{y}_n$ is the average of $y$ \ie
    \end{itemize}
 \[
\bar{y}_n= \frac{1}{n} \sum_{i=1}^I \sum_{j=1}^{n_i}y_{ij} ; i\in \llbracket 1,I \rrbracket. \]

\begin{onlyenv}<2>
\begin{itemize}
    \item  We sometimes  write : $\mu^*_i=\mu^*+\alpha^*_i $ to show the global mean effect and the specific effect of each feature.
\end{itemize}
\end{onlyenv}

\end{frame}

%%%%%%%%%%%%%%%%%%%%%%%%%%%%%%%%%%%%%%%%%%%%%%%%%%%%%%%%%%%%%%%%%%%%%%%%%%%%%%%
%%%%%%%%%%%%%%%%     Estimators in  ANOVA      %%%%%%%%%%%%%%%%%%%%%%
%%%%%%%%%%%%%%%%%%%%%%%%%%%%%%%%%%%%%%%%%%%%%%%%%%%%%%%%%%%%%%%%%%%%%%%%%%%%%%%
\begin{frame}
\rem
If we have an estimator for $\mu^*$ and $\alpha_i^*$ for all $i=1,\dots I$, noted $\hat{\mu}$ and $\hat{\alpha}$ : 

\[\hat{\mu}_i=  \hat{\mu} +  \hat{\alpha_i}  \]

and 

\begin{equation}\label{eq:sep}
(\hat{\mu}_1, \dots, \hat{\mu}_I) \in \argmin_{(\mu_1,\dots,\mu_I)\in \mathbb{R}^I} \frac{1}{2} \sum_{i=1}^I \sum_{j=1}^{n_i}(y_{ij}-\mu_i)^2
\end{equation}

\visible<2->{
\begin{alertblock}{}
Thanks to the separability principle:
\[\min_{(x_1,\dots,x_d)}f(x_1,\dots,x_d) \Longleftrightarrow \min_{x_j} g_j(x_j), \ j=1,\dots,d. \]

we have
\[\hat{\mu}_i=\frac{1}{n_i} \sum_{j=1}^{n_i}y_{ij} = \bar{y}_{i,:}.\]
\end{alertblock}
}
\end{frame}


%%%%%%%%%%%%%%%%%%%%%%%%%%%%%%%%%%%%%%%%%%%%%%%%%%%%%%%%%%%%%%%%%%%%%%%%%%%%%%%
%%%%%%%%%%%%%%%%%%%%%%      ANOVA  with the constraint sum of alpha i=0                   %%%%%%%%%%%%%%%%%%%%%%
%%%%%%%%%%%%%%%%%%%%%%%%%%%%%%%%%%%%%%%%%%%%%%%%%%%%%%%%%%%%%%%%%%%%%%%%%%%%%%%

\section{ANOVA with the constraint $\sum\alpha^*_i=0$}

\begin{frame}{ANOVA : case of a modeling with  : $\sum\alpha^*_i=0$}

\begin{itemize}\setlength{\itemsep}{5pt}
\visible<1->{\item  \textbf{hypothesis} : $\sum\limits_{i=1}^{I}\alpha_i^*=0 $ 
\medskip
We notice that if we change $\mu^*\longrightarrow \mu^*+\delta$ and $\alpha^*_i\longrightarrow \alpha^*_i-\delta$ then : $\mu_i^*=(\mu^* + \delta)+(\alpha_i^*-\delta)$}*
\visible<2->{\item \textbf{associated estimator} : $$\argmin\limits_{(\mu,\alpha)\in \mathbb{R} \times \mathbb{R}^I} \frac{1}{2} \sum\limits_{i=1}^I \sum\limits_{j=1}^{n_1}(y_{ij}-\mu - \alpha_i)^2$$}
\visible<3->{\item \textbf{Lagrangian} : $$\mathcal{L}(\mu,\alpha,\lambda)=\frac{1}{2} \sum\limits_{i=1}^I \sum\limits_{j=1}^{n_i}(y_{ij}-\mu - \alpha_i)^2 + \lambda \sum\limits_{i=1}^{I}\alpha_i $$}
\end{itemize}

\end{frame}

%%%%%%%%%%%%%%%%%%%%%%%%%%%%%%%%%%%%%%%%%%%%%%%%%%%%%%%%%%%%%%%%%%%%%%%%%%%%%%%
%%%%%%%%%%%%%%%%%%%%%%    Resolution of the optimization system                %%%%%%%%%%%%%%%%%%%%%%
%%%%%%%%%%%%%%%%%%%%%%%%%%%%%%%%%%%%%%%%%%%%%%%%%%%%%%%%%%%%%%%%%%%%%%%%%%%%%%%
\begin{frame}{Resolution of the optimization system}
\[\nabla \mathcal{L}(\hat\mu,\hat\alpha,\hat\lambda)=0\]

\[
\begin{aligned}
\begin{cases}
\sum\limits_{i=1}^{I}\hat{\alpha}_i=0 \\
\frac{\partial \mathcal{L}}{\partial \hat\mu}=0\\
\frac{\partial \mathcal{L}}{\partial \hat\alpha_{i_0}}=0\ \forall i_0
\end{cases}
\quad&\Longleftrightarrow\quad
\begin{cases}
\sum\limits_{i=1}^{I}\hat{\alpha_i}=0 \\
n\hat{\mu}+ \sum\limits_{i=1}^I n_i\hat{\alpha_i}-n\bar{y}_n=0\\
n_{i_0} \hat{\mu} +n_{i_0} \hat{\alpha_{i_0}} = \bar{y}_{i_0,:} + \hat\lambda
\end{cases} \\
& \Longleftrightarrow\quad
\begin{cases}
\displaystyle\sum_{i=1}^{I}\hat{\alpha}_i=0  \\
\hat{\mu}+\frac{1}{n} \sum\limits_{i=1}^I n_i \hat{\alpha}_i=\bar{y}_n \\
n_{i_0}(\hat{\mu}+\hat{\alpha}_{i_0}-\bar{y}_{i_0}) +\hat{\lambda}=0 
\end{cases}
\end{aligned}
\]

\end{frame}

%%%%%%%%%%%%%%%%%%%%%%%%%%%%%%%%%%%%%%%%%%%%%%%%%%%%%%%%%%%%%%%%%%%%%%%%%%%%%%%
%%%%%%%%%%%%%%%%%%%%%%    Resolution of the optimization system   continuity              %%%%%%%%%%%%%%%%%%%%%%
%%%%%%%%%%%%%%%%%%%%%%%%%%%%%%%%%%%%%%%%%%%%%%%%%%%%%%%%%%%%%%%%%%%%%%%%%%%%%%%

\begin{frame}{Resolution of the optimization system}

\vspace{0.5cm}
We have :  
$\sum\limits_{i_0 =1}^{I} n_{i_0}(\hat{\mu}+\hat{\alpha}_{i_0}-\bar{y}_{i_0,:}) +I\hat{\lambda}=0$, so for $i_0=1,\cdots,I$, so we get

\visible<2->{
\[
\begin{aligned}
& \sum_{i_0=1}^{I}n_{i_0}(\hat{\mu}+\hat{\alpha}_{i_0}-\bar{y}_{i_0}) + I\hat{\lambda}=0 \\
\Longleftrightarrow\quad & n\hat{\mu}+ \sum\limits_{i_0=1}^{I} n_{i_0}\hat{\alpha}_{i_0}- \sum\limits_{i_0=1}^{I} n_{i_0}\bar{y}_{i_0,:}+I\hat{\lambda}=0 \\
\Longleftrightarrow\quad & n\hat{\mu}+ \sum\limits_{i_0=1}^{I} n_{i_0}\hat{\alpha}_{i_0}- n\bar{y}_n+I\hat{\lambda}=0  \\
\Longleftrightarrow\quad & I\hat{\lambda}=0 \Leftrightarrow \hat{\lambda}=0 
\end{aligned}
\]}

\end{frame}


%%%%%%%%%%%%%%%%%%%%%%%%%%%%%%%%%%%%%%%%%%%%%%%%%%%%%%%%%%%%%%%%%%%%%%%%%%%%%%%
%%%%%%%%%%%%%%%%%%%%%%    Results of the optimization system                %%%%%%%%%%%%%%%%%%%%%%
%%%%%%%%%%%%%%%%%%%%%%%%%%%%%%%%%%%%%%%%%%%%%%%%%%%%%%%%%%%%%%%%%%%%%%%%%%%%%%%


\begin{frame}

\begin{alertblock}{Results: }
    \begin{itemize}
        \item $\hat{\alpha}_{i_0} + \hat{\mu}= \bar{y}_{i_0,:}$
        \item $\hat{\mu}=\dfrac{1}{I}\sum\limits_{i_0=1}^{I} \bar{y}_{i_0,:}$
    \end{itemize}

Meaning that 
\[\hat{\alpha}_{i_0}=\bar{y}_{i_0,:}-\frac{1}{I} \sum\limits_{i_0=1}^{I} \bar{y}_{i_0,:}.\]

\end{alertblock}

\begin{alertblock}{Notice: }
    \begin{itemize}
        \item $ \hat{\mu} \ne \frac{1}{n}\sum\limits_{i=1}^{I}\sum\limits_{j=1}^{n_i}y_{ij}=\bar{y}_n$
        \item It might be different if there are $ i,i'$ such that: $n_i \ne n_{i'}$
    \end{itemize}


\end{alertblock}
\end{frame}

%%%%%%%%%%%%%%%%%%%%%%%%%%%%%%%%%%%%%%%%%%%%%%%%%%%%%%%%%%%%%%%%%%%%%%%%%%%%%%%
%%%%%%%%%%%%%%%%%%%%%%     ANOVA  with the constraint sum of n i alpha i=0             %%%%%%%%%%%%%%%%%%%%%%
%%%%%%%%%%%%%%%%%%%%%%%%%%%%%%%%%%%%%%%%%%%%%%%%%%%%%%%%%%%%%%%%%%%%%%%%%%%%%%%


\section{ANOVA with the constraint $\sum\limits_{i=1}^I n_i \alpha_i=0$}
\begin{frame}{The weighted sum of the individual effects is zero}

    \begin{itemize}
        \item  \textbf{hypothesis} : \[\sum_{i=1}^{I}n_i \alpha_i=0\]\\
         
        \item \textbf{associated estimator} : \[\argmin\limits_{(\mu,\alpha)\in \mathbb{R} \times \mathbb{R}^I} \frac{1}{2} \sum_{i=1}^I \sum_{j=1}^{n_i}(y_{ij}-\mu - \alpha_i)^2\]
        \item \textbf{Lagrangian} : \[\mathcal{L}(\mu,\alpha,\lambda)=\frac{1}{2} \sum_{i=1}^I \sum_{j=1}^{n_i}(y_{ij}-\mu - \alpha_i)^2 + \lambda \sum_{i=1}^{I}n_i\alpha_i \]
    \end{itemize}



\end{frame}

%%%%%%%%%%%%%%%%%%%%%%%%%%%%%%%%%%%%%%%%%%%%%%%%%%%%%%%%%%%%%%%%%%%%%%%%%%%%%%%
%%%%%%%%%%%%%%%%%%%%%%    Resolution of the optimization system                %%%%%%%%%%%%%%%%%%%%%%
%%%%%%%%%%%%%%%%%%%%%%%%%%%%%%%%%%%%%%%%%%%%%%%%%%%%%%%%%%%%%%%%%%%%%%%%%%%%%%%

\begin{frame}{Resolution of the optimization system}
\[\nabla \mathcal{L}(\hat\mu,\hat\alpha,\hat\lambda)=0\]
\[
\begin{aligned}
\begin{cases}
&  \sum\limits_{i=1}^{I}n_i \hat{\alpha}_i=0 \\
&  \frac{\partial \mathcal{L}}{\partial \mu}=0 \\
&  \frac{\partial \mathcal{L}}{\partial \alpha_{i_0}}=0\ \forall i_0 
\end{cases}
\quad&\Longleftrightarrow\quad
\begin{cases}
&  \sum\limits_{i=1}^{I}n_i\hat{\alpha}_i=0 \\
&  n\hat{\mu}+ \sum\limits_{i=1}^I n_i\hat{\alpha}_i-n\bar{y}_n=0 \\
&  \hat{\mu}+\hat{\alpha}_{i_0}-\bar{y}_{i_0,:}+\hat{\lambda} = 0, \forall{i_0} 
\end{cases}\\
& \Longleftrightarrow\quad
\begin{cases}
& \sum\limits_{i=1}^{I}n_i \hat{\alpha}_i=0 \\
& \hat{\mu}=\bar{y}_n \\
& \hat{\alpha}_{i_0} = \bar{y}_{i_0,:}-\hat{\lambda}-\bar{y}_n

\end{cases}
\end{aligned}
\]

\end{frame}

%%%%%%%%%%%%%%%%%%%%%%%%%%%%%%%%%%%%%%%%%%%%%%%%%%%%%%%%%%%%%%%%%%%%%%%%%%%%%%%
%%%%%%%%%%%%%%%%%%%%%%    Results of the optimization system                %%%%%%%%%%%%%%%%%%%%%%
%%%%%%%%%%%%%%%%%%%%%%%%%%%%%%%%%%%%%%%%%%%%%%%%%%%%%%%%%%%%%%%%%%%%%%%%%%%%%%%

\begin{frame}

\begin{alertblock}{Results : }
    \begin{itemize}
        \item $\hat{\lambda}=0$
        \item $\hat{\mu}=\bar{y}_n$
    \end{itemize}
Meaning that:
\[\hat{\alpha}_{i_0}=\bar{y}_{i_0,:}- \bar{y}_{n}.\]
\end{alertblock}


\begin{alertblock}{Notice : }

The next case to study will be: $$ \alpha_{i_0}=0$$

\end{alertblock}

\end{frame}

%%%%%%%%%%%%%%%%%%%%%%%%%%%%%%%%%%%%%%%%%%%%%%%%%%%%%%%%%%%%%%%%%%%%%%%%%%%%%
%%%%%%%%%%%%%%%%%%%%%%%%%%    Bibliography   %%%%%%%%%%%%%%%%%%%%%%%%%%%%%%%%
%%%%%%%%%%%%%%%%%%%%%%%%%%%%%%%%%%%%%%%%%%%%%%%%%%%%%%%%%%%%%%%%%%%%%%%%%%%%%

\begin{frame}{Bibliography}
\nocite{*}
\printbibliography
\end{frame}

\end{document}